examples/paper_example_2_2.c
@@ -1,0 +1,50 @@
+// Example of Section 2.2.
+
+#include <stddef.h>
+#include <stdbool.h>
+#include <refinedc.h>
+#include <spinlock.h>
+
+// NOTE: alignment constraint hidden in a coercion.
+
+//@rc::inlined
+//@Definition layout_of_nat : nat → layout := ly_set_size struct_chunk.
+//@Coercion layout_of_nat : nat >-> layout.
+//@
+//@Close Scope Z.
+//@rc::end
+
+typedef struct
+[[rc::refined_by("s: {gmultiset nat}")]]
+[[rc::ptr_type("chunks_t : {s ≠ ∅} @ optional<&own<...>, null>")]]
+[[rc::exists  ("n : nat", "tail : {gmultiset nat}")]]
+[[rc::size    ("n")]]
+[[rc::constraints("{s = {[n]} ⊎ tail}",
+                  "{∀ k, k ∈ tail → n ≤ k}")]]
+chunk {
+  [[rc::field("n @ int<size_t>")]] size_t size;
+  [[rc::field("tail @ chunks_t")]] struct chunk* next;
+}* chunks_t;
+
+[[rc::parameters("s : {gmultiset nat}", "p : loc", "q : loc", "n : nat")]]
+[[rc::args      ("p @ &own<s @ chunks_t>", "q @ &own<uninit<n>>",
+                 "n @ int<size_t>")]]
+[[rc::requires  ("{sizeof struct_chunk ≤ n}")]]
+[[rc::ensures   ("p @ &own<{{[n]} ⊎ s} @ chunks_t>")]]
+[[rc::tactics   ("all: multiset_solver.")]]
+void free(chunks_t* list, void *data, size_t size) {
+  chunks_t *cur = list;
+  [[rc::exists  ("cp : loc", "cs : {gmultiset nat}")]]
+  [[rc::inv_vars("cur : cp @ &own<cs @ chunks_t>")]]
+  [[rc::inv_vars("list : p @ &own<"
+                   "wand<{cp ◁ₗ ({[n]} ⊎ cs) @ chunks_t}, "
+                   "{{[n]} ⊎ s} @ chunks_t>>")]]
+  while(*cur != NULL) {
+    if(size <= (*cur)->size) break;
+    cur = &(*cur)->next;
+  }
+  chunks_t entry = data;
+  entry->size = size;
+  entry->next = *cur;
+  *cur = entry;
+}
