examples/proofs/paper_example_2_1/generated_code.v
@@ -1,0 +1,253 @@
+From refinedc.lang Require Export notation.
+From refinedc.lang Require Import tactics.
+From refinedc.typing Require Import annotations.
+From refinedc.examples.spinlock Require Import spinlock_annot.
+Set Default Proof Using "Type".
+
+(* Generated from [examples/paper_example_2_1.c]. *)
+Section code.
+  Definition file_0 : string := "examples/paper_example_2_1.c".
+  Definition loc_2 : location_info := LocationInfo file_0 29 2 29 42.
+  Definition loc_3 : location_info := LocationInfo file_0 30 2 30 17.
+  Definition loc_4 : location_info := LocationInfo file_0 31 2 31 28.
+  Definition loc_5 : location_info := LocationInfo file_0 31 9 31 27.
+  Definition loc_6 : location_info := LocationInfo file_0 31 9 31 18.
+  Definition loc_7 : location_info := LocationInfo file_0 31 9 31 18.
+  Definition loc_8 : location_info := LocationInfo file_0 31 9 31 10.
+  Definition loc_9 : location_info := LocationInfo file_0 31 9 31 10.
+  Definition loc_10 : location_info := LocationInfo file_0 31 21 31 27.
+  Definition loc_11 : location_info := LocationInfo file_0 31 21 31 27.
+  Definition loc_12 : location_info := LocationInfo file_0 31 21 31 22.
+  Definition loc_13 : location_info := LocationInfo file_0 31 21 31 22.
+  Definition loc_14 : location_info := LocationInfo file_0 30 2 30 8.
+  Definition loc_15 : location_info := LocationInfo file_0 30 2 30 3.
+  Definition loc_16 : location_info := LocationInfo file_0 30 2 30 3.
+  Definition loc_17 : location_info := LocationInfo file_0 30 2 30 16.
+  Definition loc_18 : location_info := LocationInfo file_0 30 2 30 8.
+  Definition loc_19 : location_info := LocationInfo file_0 30 2 30 8.
+  Definition loc_20 : location_info := LocationInfo file_0 30 2 30 3.
+  Definition loc_21 : location_info := LocationInfo file_0 30 2 30 3.
+  Definition loc_22 : location_info := LocationInfo file_0 30 12 30 16.
+  Definition loc_23 : location_info := LocationInfo file_0 30 12 30 16.
+  Definition loc_24 : location_info := LocationInfo file_0 29 20 29 42.
+  Definition loc_25 : location_info := LocationInfo file_0 29 27 29 41.
+  Definition loc_27 : location_info := LocationInfo file_0 29 5 29 18.
+  Definition loc_28 : location_info := LocationInfo file_0 29 5 29 9.
+  Definition loc_29 : location_info := LocationInfo file_0 29 5 29 9.
+  Definition loc_30 : location_info := LocationInfo file_0 29 12 29 18.
+  Definition loc_31 : location_info := LocationInfo file_0 29 12 29 18.
+  Definition loc_32 : location_info := LocationInfo file_0 29 12 29 13.
+  Definition loc_33 : location_info := LocationInfo file_0 29 12 29 13.
+  Definition loc_36 : location_info := LocationInfo file_0 49 2 49 17.
+  Definition loc_37 : location_info := LocationInfo file_0 50 2 50 35.
+  Definition loc_38 : location_info := LocationInfo file_0 50 35 50 3.
+  Definition loc_39 : location_info := LocationInfo file_0 51 2 51 33.
+  Definition loc_40 : location_info := LocationInfo file_0 52 2 52 19.
+  Definition loc_41 : location_info := LocationInfo file_0 53 2 53 13.
+  Definition loc_42 : location_info := LocationInfo file_0 53 9 53 12.
+  Definition loc_43 : location_info := LocationInfo file_0 53 9 53 12.
+  Definition loc_44 : location_info := LocationInfo file_0 52 2 52 11.
+  Definition loc_45 : location_info := LocationInfo file_0 52 2 52 11.
+  Definition loc_46 : location_info := LocationInfo file_0 52 12 52 17.
+  Definition loc_47 : location_info := LocationInfo file_0 52 13 52 17.
+  Definition loc_48 : location_info := LocationInfo file_0 51 14 51 32.
+  Definition loc_49 : location_info := LocationInfo file_0 51 14 51 19.
+  Definition loc_50 : location_info := LocationInfo file_0 51 14 51 19.
+  Definition loc_51 : location_info := LocationInfo file_0 51 20 51 25.
+  Definition loc_52 : location_info := LocationInfo file_0 51 21 51 25.
+  Definition loc_53 : location_info := LocationInfo file_0 51 27 51 31.
+  Definition loc_54 : location_info := LocationInfo file_0 51 27 51 31.
+  Definition loc_57 : location_info := LocationInfo file_0 50 27 50 34.
+  Definition loc_58 : location_info := LocationInfo file_0 50 28 50 34.
+  Definition loc_59 : location_info := LocationInfo file_0 49 2 49 9.
+  Definition loc_60 : location_info := LocationInfo file_0 49 2 49 9.
+  Definition loc_61 : location_info := LocationInfo file_0 49 10 49 15.
+  Definition loc_62 : location_info := LocationInfo file_0 49 11 49 15.
+  Definition loc_65 : location_info := LocationInfo file_0 67 2 67 10.
+  Definition loc_66 : location_info := LocationInfo file_0 67 2 67 4.
+  Definition loc_67 : location_info := LocationInfo file_0 67 2 67 4.
+  Definition loc_68 : location_info := LocationInfo file_0 67 2 67 4.
+  Definition loc_69 : location_info := LocationInfo file_0 67 5 67 8.
+  Definition loc_70 : location_info := LocationInfo file_0 67 5 67 8.
+  Definition loc_73 : location_info := LocationInfo file_0 73 2 73 24.
+  Definition loc_74 : location_info := LocationInfo file_0 74 2 74 30.
+  Definition loc_75 : location_info := LocationInfo file_0 74 2 74 19.
+  Definition loc_76 : location_info := LocationInfo file_0 74 2 74 19.
+  Definition loc_77 : location_info := LocationInfo file_0 74 20 74 28.
+  Definition loc_78 : location_info := LocationInfo file_0 74 20 74 28.
+  Definition loc_79 : location_info := LocationInfo file_0 74 21 74 28.
+  Definition loc_80 : location_info := LocationInfo file_0 74 21 74 28.
+  Definition loc_81 : location_info := LocationInfo file_0 73 20 73 23.
+  Definition loc_82 : location_info := LocationInfo file_0 73 20 73 23.
+  Definition loc_87 : location_info := LocationInfo file_0 83 2 83 12.
+  Definition loc_88 : location_info := LocationInfo file_0 84 2 84 47.
+  Definition loc_89 : location_info := LocationInfo file_0 85 2 85 23.
+  Definition loc_90 : location_info := LocationInfo file_0 85 2 85 19.
+  Definition loc_91 : location_info := LocationInfo file_0 85 2 85 19.
+  Definition loc_92 : location_info := LocationInfo file_0 85 20 85 21.
+  Definition loc_93 : location_info := LocationInfo file_0 84 2 84 6.
+  Definition loc_94 : location_info := LocationInfo file_0 84 2 84 6.
+  Definition loc_95 : location_info := LocationInfo file_0 84 7 84 37.
+  Definition loc_96 : location_info := LocationInfo file_0 84 39 84 45.
+  Definition loc_97 : location_info := LocationInfo file_0 84 40 84 45.
+  Definition loc_98 : location_info := LocationInfo file_0 83 2 83 7.
+  Definition loc_99 : location_info := LocationInfo file_0 83 10 83 11.
+
+  (* Definition of struct [atomic_flag]. *)
+  Program Definition struct_atomic_flag := {|
+    sl_members := [
+      (Some "_Value", it_layout bool_it)
+    ];
+  |}.
+  Solve Obligations with solve_struct_obligations.
+
+  (* Definition of struct [spinlock]. *)
+  Program Definition struct_spinlock := {|
+    sl_members := [
+      (Some "lock", it_layout bool_it)
+    ];
+  |}.
+  Solve Obligations with solve_struct_obligations.
+
+  (* Definition of struct [mem_t]. *)
+  Program Definition struct_mem_t := {|
+    sl_members := [
+      (Some "len", it_layout size_t);
+      (Some "buffer", LPtr)
+    ];
+  |}.
+  Solve Obligations with solve_struct_obligations.
+
+  (* Definition of function [alloc]. *)
+  Definition impl_alloc : function := {|
+    f_args := [
+      ("d", LPtr);
+      ("size", it_layout size_t)
+    ];
+    f_local_vars := [
+    ];
+    f_init := "#0";
+    f_code := (
+      <[ "#0" :=
+        locinfo: loc_27 ;
+        if: LocInfoE loc_27 (UnOp (CastOp $ IntOp bool_it) (IntOp i32) (LocInfoE loc_27 ((LocInfoE loc_28 (use{it_layout size_t} (LocInfoE loc_29 ("size")))) >{IntOp size_t, IntOp size_t} (LocInfoE loc_30 (use{it_layout size_t} (LocInfoE loc_31 ((LocInfoE loc_32 (!{LPtr} (LocInfoE loc_33 ("d")))) at{struct_mem_t} "len")))))))
+        then
+        locinfo: loc_24 ;
+          Goto "#2"
+        else
+        locinfo: loc_3 ;
+          Goto "#3"
+      ]> $
+      <[ "#1" :=
+        locinfo: loc_3 ;
+        LocInfoE loc_14 ((LocInfoE loc_15 (!{LPtr} (LocInfoE loc_16 ("d")))) at{struct_mem_t} "len") <-{ it_layout size_t }
+          LocInfoE loc_17 ((LocInfoE loc_18 (use{it_layout size_t} (LocInfoE loc_19 ((LocInfoE loc_20 (!{LPtr} (LocInfoE loc_21 ("d")))) at{struct_mem_t} "len")))) -{IntOp size_t, IntOp size_t} (LocInfoE loc_22 (use{it_layout size_t} (LocInfoE loc_23 ("size"))))) ;
+        locinfo: loc_4 ;
+        Return (LocInfoE loc_5 ((LocInfoE loc_6 (use{LPtr} (LocInfoE loc_7 ((LocInfoE loc_8 (!{LPtr} (LocInfoE loc_9 ("d")))) at{struct_mem_t} "buffer")))) at_offset{it_layout u8, PtrOp, IntOp size_t} (LocInfoE loc_10 (use{it_layout size_t} (LocInfoE loc_11 ((LocInfoE loc_12 (!{LPtr} (LocInfoE loc_13 ("d")))) at{struct_mem_t} "len"))))))
+      ]> $
+      <[ "#2" :=
+        locinfo: loc_24 ;
+        Return (LocInfoE loc_25 (NULL))
+      ]> $
+      <[ "#3" :=
+        locinfo: loc_3 ;
+        Goto "#1"
+      ]> $∅
+    )%E
+  |}.
+
+  (* Definition of function [thread_safe_alloc]. *)
+  Definition impl_thread_safe_alloc (data lock alloc sl_lock sl_unlock : loc): function := {|
+    f_args := [
+      ("size", it_layout size_t)
+    ];
+    f_local_vars := [
+      ("ret", LPtr)
+    ];
+    f_init := "#0";
+    f_code := (
+      <[ "#0" :=
+        locinfo: loc_36 ;
+        "_" <- LocInfoE loc_60 (sl_lock) with
+          [ LocInfoE loc_61 (&(LocInfoE loc_62 (lock))) ] ;
+        locinfo: loc_37 ;
+        annot: (UnlockA) ;
+        expr: (LocInfoE loc_57 (&(LocInfoE loc_58 (data)))) ;
+        locinfo: loc_48 ;
+        "$0" <- LocInfoE loc_50 (alloc) with
+          [ LocInfoE loc_51 (&(LocInfoE loc_52 (data))) ;
+          LocInfoE loc_53 (use{it_layout size_t} (LocInfoE loc_54 ("size"))) ] ;
+        "ret" <-{ LPtr } LocInfoE loc_48 ("$0") ;
+        locinfo: loc_40 ;
+        "_" <- LocInfoE loc_45 (sl_unlock) with
+          [ LocInfoE loc_46 (AnnotExpr 1%nat LockA (LocInfoE loc_46 (&(LocInfoE loc_47 (lock))))) ] ;
+        locinfo: loc_41 ;
+        Return (LocInfoE loc_42 (use{LPtr} (LocInfoE loc_43 ("ret"))))
+      ]> $∅
+    )%E
+  |}.
+
+  (* Definition of function [fork]. *)
+  Definition impl_fork : function := {|
+    f_args := [
+      ("fn", LPtr);
+      ("arg", LPtr)
+    ];
+    f_local_vars := [
+    ];
+    f_init := "#0";
+    f_code := (
+      <[ "#0" :=
+        locinfo: loc_65 ;
+        "_" <- LocInfoE loc_67 (use{LPtr} (LocInfoE loc_68 ("fn"))) with
+          [ LocInfoE loc_69 (use{LPtr} (LocInfoE loc_70 ("arg"))) ] ;
+        Return (VOID)
+      ]> $∅
+    )%E
+  |}.
+
+  (* Definition of function [test_thread_safe_alloc_fork_fn]. *)
+  Definition impl_test_thread_safe_alloc_fork_fn (thread_safe_alloc : loc): function := {|
+    f_args := [
+      ("num", LPtr)
+    ];
+    f_local_vars := [
+      ("num_int", LPtr)
+    ];
+    f_init := "#0";
+    f_code := (
+      <[ "#0" :=
+        "num_int" <-{ LPtr }
+          LocInfoE loc_81 (UnOp (CastOp $ PtrOp) (PtrOp) (LocInfoE loc_81 (use{LPtr} (LocInfoE loc_82 ("num"))))) ;
+        locinfo: loc_74 ;
+        "_" <- LocInfoE loc_76 (thread_safe_alloc) with
+          [ LocInfoE loc_77 (use{it_layout size_t} (LocInfoE loc_79 (!{LPtr} (LocInfoE loc_80 ("num_int"))))) ] ;
+        Return (VOID)
+      ]> $∅
+    )%E
+  |}.
+
+  (* Definition of function [test_thread_safe_alloc]. *)
+  Definition impl_test_thread_safe_alloc (param fork test_thread_safe_alloc_fork_fn thread_safe_alloc : loc): function := {|
+    f_args := [
+    ];
+    f_local_vars := [
+    ];
+    f_init := "#0";
+    f_code := (
+      <[ "#0" :=
+        locinfo: loc_87 ;
+        LocInfoE loc_98 (param) <-{ it_layout size_t }
+          LocInfoE loc_99 (UnOp (CastOp $ IntOp size_t) (IntOp i32) (LocInfoE loc_99 (i2v 5 i32))) ;
+        locinfo: loc_88 ;
+        "_" <- LocInfoE loc_94 (fork) with
+          [ LocInfoE loc_95 (test_thread_safe_alloc_fork_fn) ;
+          LocInfoE loc_96 (&(LocInfoE loc_97 (param))) ] ;
+        locinfo: loc_89 ;
+        "_" <- LocInfoE loc_91 (thread_safe_alloc) with
+          [ LocInfoE loc_92 (UnOp (CastOp $ IntOp size_t) (IntOp i32) (LocInfoE loc_92 (i2v 5 i32))) ] ;
+        Return (VOID)
+      ]> $∅
+    )%E
+  |}.
+End code.
