examples/proofs/paper_example_2_2/generated_code.v
@@ -1,0 +1,163 @@
+From refinedc.lang Require Export notation.
+From refinedc.lang Require Import tactics.
+From refinedc.typing Require Import annotations.
+From refinedc.examples.spinlock Require Import spinlock_annot.
+Set Default Proof Using "Type".
+
+(* Generated from [examples/paper_example_2_2.c]. *)
+Section code.
+  Definition file_0 : string := "examples/paper_example_2_2.c".
+  Definition loc_2 : location_info := LocationInfo file_0 36 2 36 23.
+  Definition loc_3 : location_info := LocationInfo file_0 42 2 45 3.
+  Definition loc_4 : location_info := LocationInfo file_0 46 2 46 24.
+  Definition loc_5 : location_info := LocationInfo file_0 47 2 47 21.
+  Definition loc_6 : location_info := LocationInfo file_0 48 2 48 21.
+  Definition loc_7 : location_info := LocationInfo file_0 49 2 49 15.
+  Definition loc_8 : location_info := LocationInfo file_0 49 2 49 6.
+  Definition loc_9 : location_info := LocationInfo file_0 49 3 49 6.
+  Definition loc_10 : location_info := LocationInfo file_0 49 3 49 6.
+  Definition loc_11 : location_info := LocationInfo file_0 49 9 49 14.
+  Definition loc_12 : location_info := LocationInfo file_0 49 9 49 14.
+  Definition loc_13 : location_info := LocationInfo file_0 48 2 48 13.
+  Definition loc_14 : location_info := LocationInfo file_0 48 2 48 7.
+  Definition loc_15 : location_info := LocationInfo file_0 48 2 48 7.
+  Definition loc_16 : location_info := LocationInfo file_0 48 16 48 20.
+  Definition loc_17 : location_info := LocationInfo file_0 48 16 48 20.
+  Definition loc_18 : location_info := LocationInfo file_0 48 17 48 20.
+  Definition loc_19 : location_info := LocationInfo file_0 48 17 48 20.
+  Definition loc_20 : location_info := LocationInfo file_0 47 2 47 13.
+  Definition loc_21 : location_info := LocationInfo file_0 47 2 47 7.
+  Definition loc_22 : location_info := LocationInfo file_0 47 2 47 7.
+  Definition loc_23 : location_info := LocationInfo file_0 47 16 47 20.
+  Definition loc_24 : location_info := LocationInfo file_0 47 16 47 20.
+  Definition loc_25 : location_info := LocationInfo file_0 46 19 46 23.
+  Definition loc_26 : location_info := LocationInfo file_0 46 19 46 23.
+  Definition loc_29 : location_info := LocationInfo file_0 42 2 45 3.
+  Definition loc_30 : location_info := LocationInfo file_0 42 32 45 3.
+  Definition loc_31 : location_info := LocationInfo file_0 43 4 43 35.
+  Definition loc_32 : location_info := LocationInfo file_0 44 4 44 24.
+  Definition loc_33 : location_info := LocationInfo file_0 42 2 45 3.
+  Definition loc_34 : location_info := LocationInfo file_0 42 2 45 3.
+  Definition loc_35 : location_info := LocationInfo file_0 44 4 44 7.
+  Definition loc_36 : location_info := LocationInfo file_0 44 10 44 23.
+  Definition loc_37 : location_info := LocationInfo file_0 44 11 44 23.
+  Definition loc_38 : location_info := LocationInfo file_0 44 11 44 17.
+  Definition loc_39 : location_info := LocationInfo file_0 44 11 44 17.
+  Definition loc_40 : location_info := LocationInfo file_0 44 13 44 16.
+  Definition loc_41 : location_info := LocationInfo file_0 44 13 44 16.
+  Definition loc_42 : location_info := LocationInfo file_0 43 29 43 35.
+  Definition loc_44 : location_info := LocationInfo file_0 43 7 43 27.
+  Definition loc_45 : location_info := LocationInfo file_0 43 7 43 11.
+  Definition loc_46 : location_info := LocationInfo file_0 43 7 43 11.
+  Definition loc_47 : location_info := LocationInfo file_0 43 15 43 27.
+  Definition loc_48 : location_info := LocationInfo file_0 43 15 43 27.
+  Definition loc_49 : location_info := LocationInfo file_0 43 15 43 21.
+  Definition loc_50 : location_info := LocationInfo file_0 43 15 43 21.
+  Definition loc_51 : location_info := LocationInfo file_0 43 17 43 20.
+  Definition loc_52 : location_info := LocationInfo file_0 43 17 43 20.
+  Definition loc_53 : location_info := LocationInfo file_0 42 8 42 30.
+  Definition loc_54 : location_info := LocationInfo file_0 42 8 42 12.
+  Definition loc_55 : location_info := LocationInfo file_0 42 8 42 12.
+  Definition loc_56 : location_info := LocationInfo file_0 42 9 42 12.
+  Definition loc_57 : location_info := LocationInfo file_0 42 9 42 12.
+  Definition loc_58 : location_info := LocationInfo file_0 42 16 42 30.
+  Definition loc_59 : location_info := LocationInfo file_0 36 18 36 22.
+  Definition loc_60 : location_info := LocationInfo file_0 36 18 36 22.
+
+  (* Definition of struct [atomic_flag]. *)
+  Program Definition struct_atomic_flag := {|
+    sl_members := [
+      (Some "_Value", it_layout bool_it)
+    ];
+  |}.
+  Solve Obligations with solve_struct_obligations.
+
+  (* Definition of struct [spinlock]. *)
+  Program Definition struct_spinlock := {|
+    sl_members := [
+      (Some "lock", it_layout bool_it)
+    ];
+  |}.
+  Solve Obligations with solve_struct_obligations.
+
+  (* Definition of struct [chunk]. *)
+  Program Definition struct_chunk := {|
+    sl_members := [
+      (Some "size", it_layout size_t);
+      (Some "next", LPtr)
+    ];
+  |}.
+  Solve Obligations with solve_struct_obligations.
+
+  (* Definition of function [free]. *)
+  Definition impl_free : function := {|
+    f_args := [
+      ("list", LPtr);
+      ("data", LPtr);
+      ("size", it_layout size_t)
+    ];
+    f_local_vars := [
+      ("cur", LPtr);
+      ("entry", LPtr)
+    ];
+    f_init := "#0";
+    f_code := (
+      <[ "#0" :=
+        "cur" <-{ LPtr }
+          LocInfoE loc_59 (use{LPtr} (LocInfoE loc_60 ("list"))) ;
+        locinfo: loc_3 ;
+        Goto "#1"
+      ]> $
+      <[ "#1" :=
+        locinfo: loc_53 ;
+        if: LocInfoE loc_53 (UnOp (CastOp $ IntOp bool_it) (IntOp i32) (LocInfoE loc_53 ((LocInfoE loc_54 (use{LPtr} (LocInfoE loc_56 (!{LPtr} (LocInfoE loc_57 ("cur")))))) !={PtrOp, PtrOp} (LocInfoE loc_58 (NULL)))))
+        then
+        locinfo: loc_44 ;
+          Goto "#2"
+        else
+        Goto "#3"
+      ]> $
+      <[ "#2" :=
+        locinfo: loc_44 ;
+        if: LocInfoE loc_44 (UnOp (CastOp $ IntOp bool_it) (IntOp i32) (LocInfoE loc_44 ((LocInfoE loc_45 (use{it_layout size_t} (LocInfoE loc_46 ("size")))) ≤{IntOp size_t, IntOp size_t} (LocInfoE loc_47 (use{it_layout size_t} (LocInfoE loc_48 ((LocInfoE loc_49 (!{LPtr} (LocInfoE loc_51 (!{LPtr} (LocInfoE loc_52 ("cur")))))) at{struct_chunk} "size")))))))
+        then
+        Goto "#5"
+        else
+        locinfo: loc_32 ;
+          Goto "#6"
+      ]> $
+      <[ "#3" :=
+        "entry" <-{ LPtr }
+          LocInfoE loc_25 (UnOp (CastOp $ PtrOp) (PtrOp) (LocInfoE loc_25 (use{LPtr} (LocInfoE loc_26 ("data"))))) ;
+        locinfo: loc_5 ;
+        LocInfoE loc_20 ((LocInfoE loc_21 (!{LPtr} (LocInfoE loc_22 ("entry")))) at{struct_chunk} "size") <-{ it_layout size_t }
+          LocInfoE loc_23 (use{it_layout size_t} (LocInfoE loc_24 ("size"))) ;
+        locinfo: loc_6 ;
+        LocInfoE loc_13 ((LocInfoE loc_14 (!{LPtr} (LocInfoE loc_15 ("entry")))) at{struct_chunk} "next") <-{ LPtr }
+          LocInfoE loc_16 (use{LPtr} (LocInfoE loc_18 (!{LPtr} (LocInfoE loc_19 ("cur"))))) ;
+        locinfo: loc_7 ;
+        LocInfoE loc_9 (!{LPtr} (LocInfoE loc_10 ("cur"))) <-{ LPtr }
+          LocInfoE loc_11 (use{LPtr} (LocInfoE loc_12 ("entry"))) ;
+        Return (VOID)
+      ]> $
+      <[ "#4" :=
+        locinfo: loc_32 ;
+        LocInfoE loc_35 ("cur") <-{ LPtr }
+          LocInfoE loc_36 (&(LocInfoE loc_37 ((LocInfoE loc_38 (!{LPtr} (LocInfoE loc_40 (!{LPtr} (LocInfoE loc_41 ("cur")))))) at{struct_chunk} "next"))) ;
+        locinfo: loc_33 ;
+        Goto "continue2"
+      ]> $
+      <[ "#5" :=
+        Goto "#3"
+      ]> $
+      <[ "#6" :=
+        locinfo: loc_32 ;
+        Goto "#4"
+      ]> $
+      <[ "continue2" :=
+        locinfo: loc_3 ;
+        Goto "#1"
+      ]> $∅
+    )%E
+  |}.
+End code.
