examples/proofs/paper_example_2_2/generated_spec.v
@@ -1,0 +1,106 @@
+From refinedc.typing Require Import typing.
+From refinedc.examples.paper_example_2_2 Require Import generated_code.
+From refinedc.examples.spinlock Require Import spinlock_def.
+Set Default Proof Using "Type".
+
+(* Generated from [examples/paper_example_2_2.c]. *)
+Section spec.
+  Context `{!typeG Σ} `{!globalG Σ}.
+  Context `{!lockG Σ}.
+
+  (* Inlined code. *)
+
+  Definition layout_of_nat : nat → layout := ly_set_size struct_chunk.
+  Coercion layout_of_nat : nat >-> layout.
+
+  Close Scope Z.
+
+  (* Definition of type [chunks_t]. *)
+  Definition chunks_t_rec : ((gmultiset nat) -d> typeO) → ((gmultiset nat) -d> typeO) := (λ self s,
+    ((s ≠ ∅) @ (optional (&own (
+      tyexists (λ n : nat,
+      tyexists (λ tail : gmultiset nat,
+      constrained (padded (struct struct_chunk [@{type}
+        (n @ (int (size_t))) ;
+        (guarded ("chunks_t_0") (apply_dfun self (tail)))
+      ]) struct_chunk n) (
+        ⌜s = {[n]} ⊎ tail⌝ ∗
+        ⌜∀ k, k ∈ tail → n ≤ k⌝
+      )))
+    )) (null)))
+  )%I.
+  Typeclasses Opaque chunks_t_rec.
+
+  Global Instance chunks_t_rec_ne : Contractive chunks_t_rec.
+  Proof. solve_type_proper. Qed.
+
+  Definition chunks_t : rtype := {|
+    rty_type := (gmultiset nat);
+    rty r__ := fixp chunks_t_rec r__
+  |}.
+
+  Lemma chunks_t_unfold (s : gmultiset nat) :
+    (s @ chunks_t)%I ≡@{type} (
+      ((s ≠ ∅) @ (optional (&own (
+        tyexists (λ n : nat,
+        tyexists (λ tail : gmultiset nat,
+        constrained (padded (struct struct_chunk [@{type}
+          (n @ (int (size_t))) ;
+          (guarded "chunks_t_0" (tail @ chunks_t))
+        ]) struct_chunk n) (
+          ⌜s = {[n]} ⊎ tail⌝ ∗
+          ⌜∀ k, k ∈ tail → n ≤ k⌝
+        )))
+      )) (null)))
+    )%I.
+  Proof. by rewrite {1}/with_refinement/=fixp_unfold. Qed.
+
+
+  Global Program Instance chunks_t_rmovable : RMovable chunks_t :=
+    {| rmovable 's := movable_eq _ _ (chunks_t_unfold s) |}.
+  Next Obligation. solve_ty_layout_eq. Qed.
+
+  Global Instance chunks_t_simplify_hyp_place_inst l_ β_ (s : gmultiset nat) :
+    SimplifyHypPlace l_ β_ (s @ chunks_t)%I (Some 100%N) :=
+    λ T, i2p (simplify_hyp_place_eq l_ β_ _ _ T (chunks_t_unfold _)).
+  Global Instance chunks_t_simplify_goal_place_inst l_ β_ (s : gmultiset nat) :
+    SimplifyGoalPlace l_ β_ (s @ chunks_t)%I (Some 100%N) :=
+    λ T, i2p (simplify_goal_place_eq l_ β_ _ _ T (chunks_t_unfold _)).
+
+  Global Program Instance chunks_t_simplify_hyp_val_inst v_ (s : gmultiset nat) :
+    SimplifyHypVal v_ (s @ chunks_t)%I (Some 100%N) :=
+    λ T, i2p (simplify_hyp_val_eq v_ _ _ (chunks_t_unfold _) T _).
+  Next Obligation. done. Qed.
+  Global Program Instance chunks_t_simplify_goal_val_inst v_ (s : gmultiset nat) :
+    SimplifyGoalVal v_ (s @ chunks_t)%I (Some 100%N) :=
+    λ T, i2p (simplify_goal_val_eq v_ _ _ (chunks_t_unfold _) T _).
+  Next Obligation. done. Qed.
+
+  (* Type definitions. *)
+
+  (* Function [atomic_thread_fence] has been skipped. *)
+
+  (* Function [atomic_signal_fence] has been skipped. *)
+
+  (* Specifications for function [sl_init]. *)
+  Definition type_of_sl_init :=
+    fn(∀ p : loc; (p @ (&own (uninit (struct_spinlock)))); True)
+      → ∃ gamma : lock_id, (void); (p ◁ₗ (spinlock (gamma))).
+
+  (* Specifications for function [sl_lock]. *)
+  Definition type_of_sl_lock :=
+    fn(∀ (p, gamma, beta) : loc * lock_id * own_state; (p @ (&frac{beta} (spinlock (gamma)))); True)
+      → ∃ () : (), (void); (p ◁ₗ{beta} (spinlock (gamma))) ∗ (spinlock_token gamma []).
+
+  (* Specifications for function [sl_unlock]. *)
+  Definition type_of_sl_unlock :=
+    fn(∀ (p, gamma, beta) : loc * lock_id * own_state; (p @ (&frac{beta} (spinlock (gamma)))); (spinlock_token gamma []))
+      → ∃ () : (), (void); (p ◁ₗ{beta} (spinlock (gamma))).
+
+  (* Specifications for function [free]. *)
+  Definition type_of_free :=
+    fn(∀ (s, p, q, n) : (gmultiset nat) * loc * loc * nat; (p @ (&own (s @ (chunks_t)))), (q @ (&own (uninit (n)))), (n @ (int (size_t))); ⌜sizeof struct_chunk ≤ n⌝)
+      → ∃ () : (), (void); (p ◁ₗ (({[n]} ⊎ s) @ (chunks_t))).
+End spec.
+
+Typeclasses Opaque chunks_t_rec.
